Expand example to demonstrate node validity maintenance

ind/Example.fst
@@ -8,8 +8,10 @@ module DLL = DoublyLinkedListIface
 let main () : HST.Stack unit (fun _ -> True) (fun _ _ _ -> True) =
   HST.push_frame ();
   let d : DLL.dll UInt32.t = DLL.dll_new () in
-  let n = DLL.node_of 1ul in
+  let n1 = DLL.node_of 1ul in
+  let n2 = DLL.node_of 2ul in
   let h0 = HST.get () in
-  assume (DLL.fp_node n `B.loc_disjoint` DLL.fp_dll h0 d);
-  DLL.dll_insert_at_head d n;
+  assume (DLL.fp_node n1 `B.loc_disjoint` DLL.fp_dll h0 d);
+  assume (DLL.node_valid h0 n1);
+  DLL.dll_insert_at_head d n1;
   HST.pop_frame ()
